src/tls/Negotiation.Version.fst
@@ -1,13 +1,25 @@
 module Negotiation.Version
 
-open Parsers.ClientHelloExtension
 open Parsers.ProtocolVersion
-open TLSConstants
+open Parsers.ClientHelloExtension
+open TLSConstants // for leqPV and the configuration
+
+open FStar.Error
+open TLSError
 
 // updated excerpts of Negotiation re: protocol versions
 
+/// ---- PROTOCOL VERSIONS ----
+///
+/// The protocol version is negotiated in ClientHello and ServerHello,
+/// using two overlapping mechanisms.  We currently implement only TLS
+/// 1.2 and 1.3, and the negotiated version can be further constrained
+/// in the connection initial configuration.
 
-// cutting down on cases to consider after negotiation
+// 19-01-04 TODO? 
+// * replace min/max_version in config with the payload of the supported_version extension.
+// * refine TLSConstants.protocolVersion with implemented instead of not Unknown. 
+
 let implemented pv =
   pv = TLS_1p2 || pv = TLS_1p3
 
@@ -18,12 +30,10 @@ let supported cfg pv =
   cfg.min_version <= pv && pv <= cfg.max_version
 
 
-open FStar.Error
-open TLSError
-
-private let illegal #a msg: result a = fatal #a Illegal_parameter msg
-private let unsupported #a msg: result a = fatal #a Unsupported_extension msg
-
+// negotiation failures; unnecessary?
+// private let illegal       #a msg: result a = fatal #a Illegal_parameter msg
+// private let unsupported   #a msg: result a = fatal #a Unsupported_extension msg
+// private let fatal_version #a msg: result a = fatal #a Protocol_version msg
 
 /// (1) Client offers supported versions
 ///
@@ -31,30 +41,60 @@ private let unsupported #a msg: result a = fatal #a Unsupported_extension msg
 /// configuration. We may provide more flexible configurations by replacing
 /// min/max_version with a list of supported versions.
 
-#set-options "--z3rlimit 100" // 70'' to TC ?!.
+#set-options "--z3rlimit 100" // 19-01-04 too slow? note the refinement on the length of the inner lists. 
 let supported_versions cfg: option clientHelloExtension =
   match cfg.min_version, cfg.max_version with
   | TLS_1p3, TLS_1p3 -> Some (Case_supported_versions [TLS_1p3])
   | TLS_1p2, TLS_1p3 -> Some (Case_supported_versions [TLS_1p3; TLS_1p2])
   | TLS_1p2, TLS_1p2 -> Some (Case_supported_versions [TLS_1p2])
   | _                -> None
-#reset-options ""
 
+let cons_supported cfg pv pvs = if supported cfg pv then pv::pvs else pvs 
 
-/// (2) Server chooses a version
+let supported_versions2 cfg: option clientHelloExtension =
+  let vs = cons_supported cfg TLS_1p2 [] in 
+  let vs = cons_supported cfg TLS_1p3 vs in 
+  if List.isEmpty vs then None 
+  else Some(Case_supported_versions vs)
+// easier to refine and extract; worth the trouble? 
+
+(* too large?
+let same_supported cfg: Lemma (supported_versions cfg == supported_versions2 cfg) =
+  match cfg.min_version, cfg.max_version with
+  | SSL_3p0, SSL_3p0 -> assert_norm (supported_versions cfg == supported_versions2 cfg)
+  | SSL_3p0, TLS_1p0 -> assert_norm (supported_versions cfg == supported_versions2 cfg)
+  | SSL_3p0, TLS_1p1 -> assert_norm (supported_versions cfg == supported_versions2 cfg)
+  | SSL_3p0, TLS_1p2 -> assert_norm (supported_versions cfg == supported_versions2 cfg)
+  | SSL_3p0, TLS_1p3 -> assert_norm (supported_versions cfg == supported_versions2 cfg)
+  | TLS_1p0, SSL_3p0 -> assert_norm (supported_versions cfg == supported_versions2 cfg)
+  | TLS_1p0, TLS_1p0 -> assert_norm (supported_versions cfg == supported_versions2 cfg)
+  | TLS_1p0, TLS_1p1 -> assert_norm (supported_versions cfg == supported_versions2 cfg)
+  | TLS_1p0, TLS_1p2 -> assert_norm (supported_versions cfg == supported_versions2 cfg)
+  | TLS_1p0, TLS_1p3 -> assert_norm (supported_versions cfg == supported_versions2 cfg)
+  | TLS_1p1, SSL_3p0 -> assert_norm (supported_versions cfg == supported_versions2 cfg)
+  | TLS_1p1, TLS_1p0 -> assert_norm (supported_versions cfg == supported_versions2 cfg)
+  | TLS_1p1, TLS_1p1 -> assert_norm (supported_versions cfg == supported_versions2 cfg)
+  | TLS_1p1, TLS_1p2 -> assert_norm (supported_versions cfg == supported_versions2 cfg)
+  | TLS_1p1, TLS_1p3 -> assert_norm (supported_versions cfg == supported_versions2 cfg)
+  | TLS_1p2, SSL_3p0 -> assert_norm (supported_versions cfg == supported_versions2 cfg)
+  | TLS_1p2, TLS_1p0 -> assert_norm (supported_versions cfg == supported_versions2 cfg)
+  | TLS_1p2, TLS_1p1 -> assert_norm (supported_versions cfg == supported_versions2 cfg)
+  | TLS_1p2, TLS_1p2 -> assert_norm (supported_versions cfg == supported_versions2 cfg)
+  | TLS_1p2, TLS_1p3 -> assert_norm (supported_versions cfg == supported_versions2 cfg)
+  | TLS_1p3, SSL_3p0 -> assert_norm (supported_versions cfg == supported_versions2 cfg)
+  | TLS_1p3, TLS_1p0 -> assert_norm (supported_versions cfg == supported_versions2 cfg)
+  | TLS_1p3, TLS_1p1 -> assert_norm (supported_versions cfg == supported_versions2 cfg)
+  | TLS_1p3, TLS_1p2 -> assert_norm (supported_versions cfg == supported_versions2 cfg)
+  | TLS_1p3, TLS_1p3 -> assert_norm (supported_versions cfg == supported_versions2 cfg)
+*)
+
+#reset-options 
+
+/// (2) Server chooses a supported version
 ///
 /// Check that the protocol version in ClientHello is within the
 /// range of versions supported by the server configuration and
 /// outputs the negotiated version if true
-
-(*
-// no need to filter unknowns, since they can't be locally configured
-// we might also check no proposal is below min_pv
-private let rec filter_unknown_versions: list protocolVersion' -> list protocolVersion = function
-  | Unknown_protocolVersion _::vs -> filter_unknown_versions vs
-  | v::vs -> v::filter_unknown_versions vs
-  | [] -> []
-*)
 
 type offer = Parsers.ClientHello.clientHello // temporary
 
@@ -63,8 +103,9 @@ type offer = Parsers.ClientHello.clientHello // temporary
 // below the "maximal protocol version".
 
 let correct #a (x:a): result a = Correct x
-
+ 
 #set-options "--z3rlimit 100"
+val choose_version: cfg:config -> offer -> result (pv:protocolVersion{ supported cfg pv })
 let choose_version cfg offer =
   let legacy_max_pv = offer.Parsers.ClientHello.version in
   if TLS_1p3 <= legacy_max_pv then
@@ -82,10 +123,8 @@ let choose_version cfg offer =
       // new extension-based negotiation: we pick the first client offer supported by the server
       match List.Helpers.find_aux cfg supported vs with
       | Some v -> correct v
-      | None -> fatal TLSError.Protocol_version "protocol version negotiation: mismatch"
+      | None -> fatal Protocol_version "protocol version negotiation: mismatch"
 #reset-options
-// 150'' to TC?!
-
 
 /// (3) Client validates the server's choice
 
@@ -101,25 +140,17 @@ let isSentinelRandomValue client_pv server_pv server_random =
   (server_pv <= TLS_1p2 && TLS_1p3 <= client_pv && server_random = down @| abyte 1z) ||
   (server_pv <= TLS_1p1 && TLS_1p2 <= client_pv && server_random = down @| abyte 0z)
 
-let acceptable cfg (pv: Parsers.ProtocolVersion.protocolVersion) sr =
-  // we statically know that the offered versions are compatible with our config
-  // (we may prove e.g. acceptableVersion pv ==> pv in offered_versions
-  supported cfg pv &&
-  not (isSentinelRandomValue cfg.max_version pv sr)
-
-val accepted_version:
+val accept_version:
   cfg: config ->
   pv: protocolVersion ->
   ses: Parsers.ServerHello_extensions.serverHello_extensions ->
   sr: TLSInfo.random ->
-//18-12-29 wont tc?!
-//result (pv: Parsers.ProtocolVersion.protocolVersion{ acceptable cfg pv sr })
-  result Parsers.ProtocolVersion.protocolVersion
+  result (pv: Parsers.ProtocolVersion.protocolVersion{ supported cfg pv })
 
 // 18-12-23 separate protocol-version negotiation, usable as spec & implementation.
-let accepted_version cfg pv ses sr =
+let accept_version cfg pv ses sr =
   if pv = TLS_1p3 then
-    illegal "cannot negotiate TLS 1.3 explicitly"
+    fatal Illegal_parameter "cannot negotiate TLS 1.3 explicitly"
   else
     let open Parsers.ServerHelloExtension in
     let chosen: Parsers.ProtocolVersion.protocolVersion (*may be unknown*) =
@@ -127,24 +158,90 @@ let accepted_version cfg pv ses sr =
       | None -> pv // old style
       | Some (Case_supported_versions pv) -> pv in
     if TLS_1p3 <= chosen && pv <> TLS_1p2 then
-      illegal "extension-based version negotiation requires TLS 1.2 apparent version"
+      fatal Illegal_parameter "extension-based version negotiation requires TLS 1.2 apparent version"
     else
-    if acceptable cfg chosen sr then
-      correct pv
+    if isSentinelRandomValue cfg.max_version chosen sr then 
+      fatal Illegal_parameter "protocol-version downgrade attempt"
+    else 
+    if not (supported cfg chosen) then 
+      fatal Illegal_parameter "client did not offer this protocol version"
     else
-      illegal "client did not offer this protocol version"
+      correct chosen
 
-// Note TLSConstants.protocolVersion is a (not so useful) not-unknown refinement of Parsers.ProtocolVersion.protocolVersion.
-// #(pv: Parsers.ProtocolVersion.protocolVersion{ acceptable cfg pv sr })
+
+(* BEYOND VERSIONS *) 
 
 /// ----
 ///
 /// server's handling of ClientHello, a rather long stateful function.
-/// trying to write down its pure specification.
+/// calling (pure) computeServerMode, then the application callback. 
 ///
-/// effects: 
-/// 
-///
+ 
+let find_client_extension (filter:clientHelloExtension -> bool) o
+  : option (e:clientHelloExtension{filter e}) =
+  List.Tot.find filter o.Parsers.ClientHello.extensions 
+
+let find_client_key_shares (o:offer): Parsers.KeyShareClientHello.keyShareClientHello =
+  match find_client_extension Case_key_share? o with
+  | Some (Case_key_share x) -> x
+  | _ -> assume(Parsers.KeyShareClientHello.keyShareClientHello_list_bytesize [] = 0); []
+//TODO 19-01-04 where to get it from? 
+
+let group_of_hrr hrr : option CommonDH.group = None
+//19-01-03 TODO where are QD's HRR extensions? 
+(*
+  match List.Tot.find (Extensions.E_key_share?) hrr.hrr_extensions with
+  | Some (Extensions.E_key_share (CommonDH.HRRKeyShare ng)) ->
+    CommonDH.group_of_namedGroup ng
+  | _ -> None
+*)
+
+private
+let sameExtensionTag e0 e1 = tag_of_clientHelloExtension e0 = tag_of_clientHelloExtension e1 
+
+private
+let retry_extension_ok (o1, hrr) (e:clientHelloExtension) = 
+  match e with
+// 19-01-04 TODO   
+// | Case_key_share shares2 -> (
+//     match shares2, group_of_hrr hrr with
+//     | [CommonDH.Share g _], Some g' -> g = g'
+//     | _, None ->
+//         let shares1 = find_client_key_shares o1 in
+//         //TODO 19-01-03 easier on the underlying wire representation
+//         Parsers.KeyShareClientHello.keyShareClientHello_serializer32 shares1 =
+//         Parsers.KeyShareClientHello.keyShareClientHello_serializer32 shares2
+//         // CommonDH.clientKeyShareBytes shares1 = CommonDH.clientKeyShareBytes shares2
+//     | _ -> false)
+  | Case_early_data _ -> false // Forbidden
+  | Case_cookie c -> true // FIXME we will send cookie
+      // If we add cookie support we need to treat this case separately
+      // | Extensions.E_cookie c -> c = S_HRR?.cookie ns.state
+  | e ->
+        (match List.Helpers.find_aux e sameExtensionTag o1 with
+        | None -> (IO.debug_print_string "Extra extension\n") && false
+        // This allows the client to send less extensions,
+        // but the ones that are sent must be exactly the same
+        | Some e' ->
+          //FIXME: Extensions.E_pre_shared_key "may be updated" 4.1.2
+          true) // FIXME
+          //(extensionBytes e) = (extensionBytes e'))
+
+// check the second offer is compatible with the first (see RFC)
+let retry_offer_ok o1 hrr o2 = 
+  let open Parsers.ClientHello in 
+  o1.version = o2.version &&
+  o1.random = o2.random &&
+  o1.session_id = o2.session_id &&
+// TODO 19-01-04 
+//  o1.session_id = hrr.hrr_sessionID &&
+//  List.Tot.mem hrr.hrr_cipher_suite o2.ch_cipher_suites &&
+  o1.compression_method = o2.compression_method &&
+  List.Helpers.forall_aux (o1.extensions, hrr) retry_extension_ok o2.extensions
+
+open Mem 
+
+(*
 val server_ClientHello: // #region:rgn -> t region Server ->
   offer -> // log:HandshakeLog.t ->
   St (result serverMode)
@@ -157,22 +254,8 @@ let server_ClientHello #region ns offer log =
         | Correct v -> List.Tot.fold_left accum_string_of_pv "offered versions" v);
   match !ns.state with
   | S_HRR o1 hrr ->
-    trace ("Processing second offer based on existing HRR state (staeful HRR).");
-    let o2 = offer in
-    let extension_ok =
-      if Some? o2.ch_extensions && Some? o1.ch_extensions then
-        List.Helpers.forall_aux (o1, hrr) aux_extension_ok (Some?.v o2.ch_extensions)
-      else
-        false
-    in
-    if
-      o1.ch_protocol_version = o2.ch_protocol_version &&
-      o1.ch_client_random = o2.ch_client_random &&
-      o1.ch_sessionID = o2.ch_sessionID &&
-      o1.ch_sessionID = hrr.hrr_sessionID &&
-      List.Tot.mem hrr.hrr_cipher_suite o2.ch_cipher_suites &&
-      o1.ch_compressions = o2.ch_compressions &&
-      extension_ok
+    trace ("Processing second offer based on existing HRR state (stateful HRR).");
+    if retry_offer_ok o1 offer
     then
       let sm = computeServerMode ns.cfg offer ns.nonce in
       match sm with
@@ -196,6 +279,7 @@ let server_ClientHello #region ns offer log =
           fatal Handshake_failure "application aborted the handshake by callback"
     else
       fatal Illegal_parameter "Inconsistant parameters between first and second client hello"
+
   | S_Init _ ->
     let sm = computeServerMode ns.cfg offer ns.nonce in
     let previous_cookie = // for stateless HRR
@@ -255,3 +339,4 @@ let server_ClientHello #region ns offer log =
         trace ("negotiated "^string_of_pv m.n_protocol_version^" "^string_of_ciphersuite m.n_cipher_suite);
         ns.state := S_ClientHello m cert;
         Correct (ServerMode m cert (Extensions.ext_of_custom sexts))
+*)
